Grandpa/src/DataTypes/NatWrapper.v
@@ -7,6 +7,37 @@ Require Import Classes.Math.All.
 Declare Scope natWrapper_scope.
 Delimit Scope natWrapper_scope with natWrapper.
 
+(** *NatWrapper
+Coq doesn't have support for [newtypes], instead we 
+must create a regular type every time we want to 
+wrap some type around.
+
+The case of wrapping a natural is a recurrent pattern.
+
+Two important types that use this wrapper are:
+  - Time
+  - Round
+*)
+
+
+(**
+  The type [T] is a phantom type, it's only use is to distinguish two 
+   different natural wrappers, otherwise we would defeat the entire 
+   purpose of using a wrapper.
+
+  This means that every time you want to create a natural wrapper you
+   need to create a phantom type representing it first. 
+
+  A minimal definition of a wrapper in a new module looks like this:
+
+   [
+    Require Import NatWrapper.
+
+    Variant CustomCounterPhantom := CustomCounterPhantomC.
+    Definition CustomCounter := NatWrapper CustomCounterPhantom
+    Definition from_nat n : CustomCounter := NatWrapper.from_nat n
+   ]
+*)
 Record NatWrapper (T:Type) :Type 
     := NatWrapperC { to_nat:nat }.
 
@@ -135,6 +166,10 @@ Infix "-" := (fun x y => from_nat ((to_nat x) - (to_nat y))) : natWrapper_scope.
 #[global]
 Infix "*" := (fun x y => from_nat ((to_nat x) * (to_nat y))) : natWrapper_scope.
 
+(*
+TODO: The proper way to adquire this notation must be by defining boolean 
+ordering classes as we did with Eqb.
+*)
 #[global]
 Infix "<" := (fun x y => ((to_nat x) < (to_nat y)))%nat : natWrapper_scope.
 
