Grandpa/src/Protocol/Protocol.v
@@ -11,6 +11,7 @@ Require Import Vectors.
 Require Import Sets.
 Require Import Message.
 Require Import DataTypes.List.Count.
+Require Import DataTypes.Option.
 Require Import Protocol.State.
 Require Import Protocol.StateMessages.
 Require Import Protocol.FinalizedBlock.
@@ -36,24 +37,77 @@ Open Scope eqb.
 Open Scope math.
 Open Scope natWrapper.
 
+(** *Protocol
 
+The main functions of this module are: 
+  - [get_state_up_to]
+  - [voters_round_step]
+
+Of the same importance but no defined in this module is the 
+  [StateMessages.update_votes] function.
+
+The [get_state_up_to] function is in charge of performing the 
+main loop of the simulation. It just take the 0 state 
+and feed the [voter_round_step] and  [StateMessages.update_votes] functions 
+with the right states for the corresponding [Time] until 
+we reach the desired Time.
+
+At every time [t], we have two stages:  
+  - Update the local state of every voter according to the messages received 
+    by that voter up to this time. 
+  - Proceed to run the Grandpa protocol or to act as a byzantine voter 
+    for every voter of the protocol.
+
+The [StateMessages.update_votes] function models the message passing 
+between participants. 
+
+The [voters_round_step] function models the actions of the participants 
+at a particular time and global state of the protocol.
+
+See the documentation of each function for details.
+
+Other functions of high interest: 
+
+  - [prevoter_step_legit] what a honest prevoter does 
+  - [precommit_step_legit] what a honest precommiter does
+  - [finalize_block]
+*)
+
+
+(**
+Given a block [b], looks in all the blocks produced by block producer 
+for this round and time.
+Filters all the blocks [x] such that [b <=? x].
+And gets the block with the higher block number.
+*)
 Definition look_for_best_chain_for_block `{Io} (t:Time) (v:Voter) (ablock:AnyBlock)
-  : AnyBlock
+  : option AnyBlock
   :=
   let (block_number,block) := ablock
   in
   let available_blocks := block_producer t v
   in
-    List.fold_left 
-      (fun x y => if (x.(AnyBlock.block_number) <? y.(AnyBlock.block_number))%nat then y else x)
-      (
-        List.filter 
-        (fun x => Block.is_prefix block  x.(AnyBlock.block)) 
-        (Sets.to_list available_blocks)
-      )
-      (AnyBlock.to_any OriginBlock).
+  let blocks_that_contains_it := 
+    List.filter 
+    (fun x => AnyBlock.is_prefix ablock  x) 
+    (Sets.to_list available_blocks)
+  in
+  match blocks_that_contains_it with
+  | List.nil => None
+  | _ =>
+    Some(
+      List.fold_left 
+        (fun x y => if (x.(AnyBlock.block_number) <? y.(AnyBlock.block_number))%nat then y else x)
+        blocks_that_contains_it
+        (AnyBlock.to_any OriginBlock)
+    )
+  end.
 
-
+(**
+Creates a prevote message for the given block, 
+adds it to the local state (to set that the voter already voted),
+and sends the message.
+*)
 Definition build_and_send_prevote
   (t:Time)
   (state:State) 
@@ -82,6 +136,11 @@ Definition build_and_send_prevote
         advance_count
           (update_voter_state (update_message state new_message) voter up_round).
 
+(**
+Creates a precommit message for the given block, 
+adds it to the local state (to set that the voter already voted),
+and sends the message.
+*)
 Definition build_and_send_precommit
   (t:Time)
   (state:State) 
@@ -140,6 +199,12 @@ Definition build_and_send_primary_estimate
             voter updated_voter_state
           ).
 
+
+(**
+Create a message that the given block is being finalized, 
+adds it to the local collection of finalized blocks, 
+and send the message.
+*)
 Definition build_and_send_finalized_block
   (t:Time)
   (state:State) 
@@ -191,8 +256,8 @@ Definition prevoter_step_aux `{Io} (t:Time) (state:State) (voter:Voter) (vs:Vote
           | (Some g_prev, Some estimate_prev)
               =>
               if 
-                is_prefix estimate_prev.(AnyBlock.block) b.(AnyBlock.block) 
-                && is_prefix b.(AnyBlock.block) g_prev.(AnyBlock.block)
+                Block.is_prefix estimate_prev.(AnyBlock.block) b.(AnyBlock.block) 
+                && Block.is_prefix b.(AnyBlock.block) g_prev.(AnyBlock.block)
               then Some b
               else Estimate.get_estimate previous_round
           | _ => Estimate.get_estimate previous_round
@@ -201,8 +266,8 @@ Definition prevoter_step_aux `{Io} (t:Time) (state:State) (voter:Voter) (vs:Vote
       end
     in 
     match map (look_for_best_chain_for_block t voter) ref_block with 
-    | Some b => build_and_send_prevote t state voter vs b
-    | None => state
+    | Some (Some b) => build_and_send_prevote t state voter vs b
+    | _ => state
     end
   | None => state
   end.
@@ -323,6 +388,11 @@ Definition get_last_finalized_block_number
     (Sets.to_list finalized_blocks)
     0.
 
+(**
+A block $b = g (C_{r,v})$ can be finalized by a voter [v] if : 
+  - [b] its block number is above the all the finalized blocks the voter knows.
+  - [b] has a supermajority in $V_{r,v}$
+*)
 Definition should_finalize
   (finalized_blocks:Sets.DictionarySet AnyBlock)  
   (opaque:OpaqueRound.OpaqueRoundState) 
@@ -341,23 +411,13 @@ Definition should_finalize
           (fun b2 
             => 
             (b.(AnyBlock.block_number) <? max_block_number)%nat
-            ||
-            is_prefix b.(AnyBlock.block) b2.(AnyBlock.block)
           ) 
           finalized_blocks
-        )
+        ) && Votes.block_has_supermajority b (Round.get_all_prevote_votes r)
       then 
         Some b 
       else None
     end
-  end.
-
-
-Definition is_some {A} (o:option A) : bool
-  := 
-  match o with 
-  | Some _ => true
-  | _ => false
   end.
 
 Definition get_voter_kind_for_round `{Io} (v:Voter) (round_number:RoundNumber)
@@ -375,6 +435,16 @@ Definition is_voter_for_round `{Io} (v:Voter) (round_number:RoundNumber)
   := 
   is_some (get_voter_kind_for_round v round_number).
 
+(**
+All the blocks on all the rounds that a voter can finalize that haven 
+been finalized.
+
+First, we get all the blocks that the current voter knows has been finalized.
+Then get all the rounds in witch the current voter has participated 
+until now.
+We inspect every round to see if we can finalize now a block that haven been 
+finalized before.
+*)
 Program Definition get_blocks_to_finalize `{Io} (voter:Voter) (vs:VoterState) 
   : list (OpaqueRound.OpaqueRoundState * AnyBlock)
   := 
@@ -416,6 +486,11 @@ Next Obligation.
   apply PeanoNat.Nat.le_succ_diag_r.
 Qed.
 
+(**
+Made to me used together with get_blocks_to_finalize.
+Take a block and all the info needed to build a [FinalizedBlock],
+then adds it to the finalized_blocks in the global state.
+*)
 Definition finalize_block (t:Time) 
   (voter:Voter) 
   (state:State) 
@@ -440,7 +515,10 @@ Definition finalize_block (t:Time)
   | None => state
   end.
  
-
+(**
+Multiple voters may finalize the same block if they notice it can be 
+finalized but haven't received a finalization message.
+*)
 Definition finalization `{Io} (t:Time) (state:State) 
   (voter:Voter) (vs:VoterState) 
   :State 
@@ -451,6 +529,10 @@ Definition finalization `{Io} (t:Time) (state:State)
     state.
 
 
+(**
+See if the current round is completable and advance to next round in such case.
+If voter is the primary voter, we also broadcast the estimate.
+*)
 Definition wait_step_for_new_round `{Io}
   (t:Time) 
   (voter:Voter) 
@@ -517,6 +599,19 @@ Definition should_wait_for_next_round `{Io}
   | None => true
   end.
 
+
+(**
+If the participant (voter) has one of 
+the following conditions ([should_wait_for_next_round]):
+   - Is a byzantine voter wishing to advance round.
+   - Is a voter that already fulfilled it's obligations for this round.
+   - Isn't a voter for this round.
+We see if the current round (for the voter) is completable and if it is, 
+we advance the voter local state to a new round. Otherwise do nothing.
+
+Otherwise we get perform the corresponding action for the particular voter
+in the protocol or the byzantine action.
+*)
 Definition voter_round_step_aux `{Io} (t:Time) (state:State) (voter:Voter): State :=
   match get_voter_state voter state with
   | Some voter_state_ =>  
@@ -553,8 +648,21 @@ Definition voter_round_step_aux `{Io} (t:Time) (state:State) (voter:Voter): Stat
   | _ => state
   end.
 
+(**
+First we attempt to finalize all the blocks that we see as finalized but 
+that aren't still finalized by some one.
+
+Then we really perform the Grandpa protocol or the byzantiner actions for 
+this time.
+*)
+(*TODO:
+If this function is called by the members of voters_round_step, 
+the lookup for the voter must be always a Some. This is guaranteed by 
+the facts in the Io class and the way we construct the states. 
+We may add a theorem stating this. 
+*)
 Definition voter_round_step `{Io} (t:Time) (state:State) (voter:Voter): State :=
-  match Dictionary.lookup voter state.(voters_state)with
+  match get_voter_state voter state with
   | Some vs =>  
     voter_round_step_aux 
       t 
@@ -563,52 +671,60 @@ Definition voter_round_step `{Io} (t:Time) (state:State) (voter:Voter): State :=
   | None => state
   end.
 
+(** 
+This function models the grandpa protocol together with byzantine voters.
+
+If a particular participant is byzantine in a round, they send messages 
+as dictated by the functions in Io. 
+
+If a participant is honest in a round, it follows the grandpa protocol.
+
+This function expect to be run after a votes update. 
+This means that all participants of the model have received all the 
+messages that they are supposed to receive at this time.
+
+As we separate the process of reception of votes/messages from the emission 
+of them, we can update every voter local state independently. 
+This update for a single voter is done in [voter_round_step].
+*)
 Definition voters_round_step `{Io} (t:Time) (state:State): State :=
   let voters := List.map fst (Dictionary.to_list state.(voters_state))
   in 
     List.fold_left (voter_round_step t) voters state .
 
 
-
-CoInductive CoList (T:Type) :Type :=
-  | CoCons : T -> CoList T -> CoList T.
-
-Arguments CoCons {T}.
-
-Fixpoint get_last_nat_aux {T} (n:nat) (colist:CoList T): T
-  := 
+Fixpoint get_state_up_to_nat_aux `{Io} (n:nat) (state_0:State) 
+  : State 
+  :=
   match n with 
-  | 0 => match colist  with 
-         | CoCons element _ =>
-             element
-          end
-  | S m => match colist with 
-          | CoCons _ remain => get_last_nat_aux m remain
-          end
+  | 0 => state_0
+  | S m 
+    => 
+    let old_state := get_state_up_to_nat_aux m state_0
+    in
+    voters_round_step 
+      (Time.from_nat n) 
+      (update_votes (Time.from_nat n) old_state)
   end.
 
-Definition get_last {T} (t:Time) (colist:CoList T): T
-  := get_last_nat_aux (Time.to_nat t) colist.
-
-
-CoFixpoint produce_states `{Io} (t:Time) (state:State): CoList State :=
-  let new_state := voters_round_step t (update_votes t state)
-  in
-  CoCons state  (produce_states (Time.from_nat 1 +t) new_state).
-
-
-Definition get_state_up_to `{Io} (t:Time): State :=   
+Definition get_state_up_to `{Io} (t:Time) : State 
+  :=
   let 
     zero_round_dict := io_get_round_voters (RoundNumber.from_nat 0)
   in
-  get_last t 
-  (
-    produce_states 
-      (Time.from_nat 0) 
-      (State.make_initial_state_from zero_round_dict)
-  ). 
+  let 
+    state_0 :=  State.make_initial_state_from zero_round_dict
+  in
+  get_state_up_to_nat_aux (Time.to_nat t) state_0.
 
-(*Compute get_state_up_to (Time.from_nat 0).*)
+
+(*
+This takes some time to compute, but it eventually does.
+We believe the reason is that no Io instance is provide and the 
+computation must be made abstract. As such, we end with a 300k 
+lines result instead of a simple State.
+*)
+(* Compute get_state_up_to (Time.from_nat 1).*)
 
 
 Lemma get_global_finalized_blocks_are_related (state:State)
