Grandpa/src/Message.v
@@ -25,6 +25,12 @@ Definition from_nat := @NatWrapper.from_nat MessageIdPhantom.
 Definition to_nat := @NatWrapper.to_nat MessageIdPhantom.
 
 
+(**
+  The evidence of the voter sending the message 
+   to include the block as finalized.
+
+  A byzantine voter may send anything.
+*)
 Record FinalizeBlock :Type 
   :=
   {
@@ -35,12 +41,40 @@ Record FinalizeBlock :Type
   }.
 
 
+
+
+(**
+  The FinalizationMessage inducles a parameter as a hack to 
+   store the voter evidence.
+*)
 Variant MessageKind : Type
   :=
   | PreCommitMessage : MessageKind
   | PreVoteMessage : MessageKind
   | EstimateMessage: MessageKind
   | FinalizationMessage (votes:FinalizeBlock) : MessageKind.
+
+(**
+In a real implementation we may distinguish messages by the 
+id of the voter is sending it and another id related to it 
+(maybe they mantain their own or we use a hash).
+
+Whoever our model runs in a single machine and allow us to 
+maintain the notion of _the total number of messages emitted_ .
+
+The message include all the information to recognize who send it,
+at what time was send and the round at witch this message correspond.
+
+For messages we maintain a single global collection storing all the 
+messages that haven't been received by all voters. 
+
+We attempt to deliver a message to all the participants that haven't receive it 
+before we start a step in the main model loop. 
+As such, every message stores the set of voters that have received it until now.
+
+Whenever a message [processed_by] field contains all the protocol participants, 
+we delete the message from the global collection of messages.
+*)
 
 Record Message :=
    { id:MessageId
